src/Init/Data/Iterators/Lemmas/Combinators/Monadic/Attach.lean
@@ -22,10 +22,10 @@ theorem IterM.step_attachWith [Iterator α m β] [Monad m] {it : IterM (α := α
   rfl
 
 @[simp]
-theorem IterM.map_unattach_toList_attachWith [Iterator α m β] [Monad m]
-    {it : IterM (α := α) m β} {hP}
-    [Finite α m] [IteratorCollect α m m]
-    [LawfulMonad m] [LawfulIteratorCollect α m m] :
+theorem IterM.map_unattach_toList_attachWith [Iterator α m β]
+    [Monad m] [MonadAttach m] [LawfulMonad m] [LawfulMonadAttach m]
+    [Finite α m] [IteratorCollect α m m] [LawfulIteratorCollect α m m]
+    {it : IterM (α := α) m β} {hP} :
     List.unattach <$> (it.attachWith P hP).toList = it.toList := by
   induction it using IterM.inductSteps with | step it ihy ihs
   rw [IterM.toList_eq_match_step, IterM.toList_eq_match_step, step_attachWith]
@@ -42,19 +42,19 @@ theorem IterM.map_unattach_toList_attachWith [Iterator α m β] [Monad m]
   · simp [Types.Attach.Monadic.modifyStep]
 
 @[simp]
-theorem IterM.map_unattach_toListRev_attachWith [Iterator α m β] [Monad m] [Monad n]
-    {it : IterM (α := α) m β} {hP}
-    [Finite α m] [IteratorCollect α m m]
-    [LawfulMonad m] [LawfulIteratorCollect α m m] :
+theorem IterM.map_unattach_toListRev_attachWith [Iterator α m β]
+    [Monad m] [MonadAttach m] [LawfulMonad m] [LawfulMonadAttach m] [Monad n]
+    [Finite α m] [IteratorCollect α m m] [LawfulIteratorCollect α m m]
+    {it : IterM (α := α) m β} {hP} :
     List.unattach <$> (it.attachWith P hP).toListRev = it.toListRev := by
   rw [toListRev_eq, toListRev_eq, ← map_unattach_toList_attachWith (it := it) (hP := hP)]
   simp [-map_unattach_toList_attachWith]
 
 @[simp]
-theorem IterM.map_unattach_toArray_attachWith [Iterator α m β] [Monad m] [Monad n]
-    {it : IterM (α := α) m β} {hP}
-    [Finite α m] [IteratorCollect α m m]
-    [LawfulMonad m] [LawfulIteratorCollect α m m] :
+theorem IterM.map_unattach_toArray_attachWith [Iterator α m β]
+    [Monad m] [MonadAttach m] [LawfulMonad m] [LawfulMonadAttach m] [Monad n]
+    [Finite α m] [IteratorCollect α m m] [LawfulIteratorCollect α m m]
+    {it : IterM (α := α) m β} {hP} :
     (·.map Subtype.val) <$> (it.attachWith P hP).toArray = it.toArray := by
   rw [← toArray_toList, ← toArray_toList, ← map_unattach_toList_attachWith (it := it) (hP := hP)]
   simp [-map_unattach_toList_attachWith, -IterM.toArray_toList]
