src/Std/Data/Iterators/Combinators/Monadic/Drop.lean
@@ -152,7 +152,8 @@ instance Drop.instProductive [Iterator α m β] [Monad m] [Productive α m] :
     Productive (Drop α m β) m :=
   by exact Productive.of_productivenessRelation instProductivenessRelation
 
-instance Drop.instIteratorCollect {n : Type w → Type w'} [Monad m] [Monad n] [Iterator α m β] [Finite α m] :
+instance Drop.instIteratorCollect {n : Type w → Type w'}
+    [Monad m] [MonadAttach m] [Monad n] [MonadAttach n] [Iterator α m β] [Finite α m] :
     IteratorCollect (Drop α m β) m n :=
   .defaultImplementation
 
