src/Std/Data/Iterators/Lemmas/Combinators/Monadic/Take.lean
@@ -30,9 +30,10 @@ theorem IterM.step_take {α m β} [Monad m] [Iterator α m β] {n : Nat}
     intro step
     cases step.inflate using PlausibleIterStep.casesOn <;> rfl
 
-theorem IterM.toList_take_zero {α m β} [Monad m] [LawfulMonad m] [Iterator α m β]
-    [Finite (Take α m β) m]
-    [IteratorCollect (Take α m β) m m] [LawfulIteratorCollect (Take α m β) m m]
+theorem IterM.toList_take_zero {α m β}
+    [Monad m] [MonadAttach m] [LawfulMonad m] [LawfulMonadAttach m] [Iterator α m β]
+    [Finite (Take α m β) m] [IteratorCollect (Take α m β) m m]
+    [LawfulIteratorCollect (Take α m β) m m]
     {it : IterM (α := α) m β} :
     (it.take 0).toList = pure [] := by
   rw [toList_eq_match_step]
