src/Std/Data/Iterators/Lemmas/Consumers/Monadic/Collect.lean
@@ -35,7 +35,8 @@ theorem IterM.Equiv.toListRev_eq [Monad m] [LawfulMonad m]
     exact BundledIterM.Equiv.exact _ _ h
   · simp
 
-theorem IterM.Equiv.toList_eq {α₁ α₂ : Type w} {m : Type w → Type w'} [Monad m] [LawfulMonad m]
+theorem IterM.Equiv.toList_eq {α₁ α₂ β : Type w} {m : Type w → Type w'}
+    [Monad m] [MonadAttach m] [LawfulMonad m] [LawfulMonadAttach m]
     [Iterator α₁ m β] [Iterator α₂ m β] [Finite α₁ m] [Finite α₂ m]
     [IteratorCollect α₁ m m] [LawfulIteratorCollect α₁ m m]
     [IteratorCollect α₂ m m] [LawfulIteratorCollect α₂ m m]
@@ -43,7 +44,8 @@ theorem IterM.Equiv.toList_eq {α₁ α₂ : Type w} {m : Type w → Type w'} [M
     ita.toList = itb.toList := by
   simp only [← IterM.reverse_toListRev, toListRev_eq h]
 
-theorem IterM.Equiv.toArray_eq [Monad m] [LawfulMonad m]
+theorem IterM.Equiv.toArray_eq {α₁ α₂ β : Type w} {m : Type w → Type w'}
+    [Monad m] [MonadAttach m] [LawfulMonad m] [LawfulMonadAttach m]
     [Iterator α₁ m β] [Iterator α₂ m β] [Finite α₁ m] [Finite α₂ m]
     [IteratorCollect α₁ m m] [LawfulIteratorCollect α₁ m m]
     [IteratorCollect α₂ m m] [LawfulIteratorCollect α₂ m m]
